\subsection*{الف}

$$
L_x (c) = |x - c|
$$

$$
\rightarrow \int_{c}^{\infty} f_x(x) (x - c) \, dx + \int_{- \infty}^{c} f_x(x) (c - x) \, dx
$$

$$
= - (1 - F_x(c)) + F_x(c) = 2 F_x(c) - 1 = 0
$$

$$
\rightarrow c = F^{-1}_x (\frac{1}{2})
$$

\subsection*{ب}

$$
L_x (c) = (x - c)^2
$$

$$
\rightarrow \int_{- \infty}^{\infty} (x - c)^2 \, dx
$$

$$
= 2c - 2E[x] = 0 \rightarrow c = E[x]
$$

\subsection*{ج}

برای این بخش نیز داریم:

$$
\int_{- \infty}^{c} f_x(x) k (c - x) \, dx + \int_{c}^{\infty} f_x(x)(x - c) \, dx = 0
$$

$$
\rightarrow F_x(c) = \frac{1}{k+1}
$$

$$
c = F^{-1}_x \frac{1}{k+1}
$$
